code/ecdsap256/Hacl.Impl.P256.Compression.fsti
@@ -12,79 +12,31 @@ module S = Spec.P256
 
 #set-options "--z3rlimit 30 --fuel 0 --ifuel 0"
 
-let notCompressedForm = lbuffer uint8 (size 65)
-let compressedForm = lbuffer uint8 (size 33)
+inline_for_extraction noextract
+val uncompressed_to_raw: pk:lbuffer uint8 65ul -> pk_raw:lbuffer uint8 64ul -> Stack bool
+  (requires fun h -> live h pk /\ live h pk_raw /\ disjoint pk pk_raw)
+  (ensures fun h0 b h1 -> modifies (loc pk_raw) h0 h1 /\
+    (b <==> Some? (S.pk_uncompressed_to_raw (as_seq h0 pk))) /\
+    (b ==> (as_seq h1 pk_raw == Some?.v (S.pk_uncompressed_to_raw (as_seq h0 pk)))))
 
-inline_for_extraction
-val decompressionNotCompressedForm: b: notCompressedForm -> result: lbuffer uint8 (size 64) -> Stack bool
-  (requires fun h -> live h b /\ live h result /\ disjoint b result)
-  (ensures fun h0 r h1 -> modifies (loc result) h0 h1 /\
-    (
-      let id = Lib.Sequence.index (as_seq h0 b) 0 in
-      let x = Lib.Sequence.sub (as_seq h0 b) 1 32 in
-	let xResult = Lib.Sequence.sub (as_seq h1 result) 0 32 in
-      let y = Lib.Sequence.sub (as_seq h0 b) 33 32 in
-	let yResult = Lib.Sequence.sub (as_seq h1 result) 32 32 in
-	  if uint_v id = 4 then
-	    r == true /\ x == xResult /\ y == yResult
-  	  else
-	    r == false
-  	)
-)
 
-inline_for_extraction
-val decompressionCompressedForm: b: compressedForm -> result: lbuffer uint8 (size 64) -> Stack bool
-  (requires fun h -> live h b /\ live h result /\ disjoint b result)
-  (ensures fun h0 r h1 ->
-    (
-      let id = Lib.Sequence.index (as_seq h0 b) 0 in
-      let xSequence = Lib.Sequence.sub (as_seq h0 b) 1 32 in
-      let x =  Lib.ByteSequence.nat_from_bytes_be xSequence in
-      if uint_v id = 2 || uint_v id = 3 then
-	if x < S.prime then
-	  r == true /\
-	  (
-	    let y =
-              let sq = S.fsqrt (((x * x * x + Spec.P256.a_coeff * x + Spec.P256.b_coeff) % S.prime)) in
-              if (uint_v id) % 2 = (sq % 2) then
-		sq
-              else
-	         (0 - sq) % S.prime
-	    in
-	    as_seq h1 (gsub result (size 0) (size 32)) == xSequence /\
-	    as_seq h1 (gsub result (size 32) (size 32)) == Lib.ByteSequence.nat_to_bytes_be 32 y)
-	else
-	  r == false
-      else
-	r == false) /\
-  modifies (loc result) h0 h1)
+inline_for_extraction noextract
+val compressed_to_raw: pk:lbuffer uint8 33ul -> pk_raw:lbuffer uint8 64ul -> Stack bool
+  (requires fun h -> live h pk /\ live h pk_raw /\ disjoint pk pk_raw)
+  (ensures  fun h0 b h1 -> modifies (loc pk_raw) h0 h1 /\
+    (b <==> Some? (S.pk_compressed_to_raw (as_seq h0 pk))) /\
+    (b ==> (as_seq h1 pk_raw == Some?.v (S.pk_compressed_to_raw (as_seq h0 pk)))))
 
-inline_for_extraction
-val compressionNotCompressedForm: b: lbuffer uint8 (size 64) -> result: notCompressedForm ->
-  Stack unit
-    (requires fun h -> live h b /\ live h result /\ disjoint b result)
-    (ensures fun h0 _ h1 -> modifies (loc result) h0 h1 /\
-      (
-	let id = Lib.Sequence.index (as_seq h1 result) 0 in
-	let x = Lib.Sequence.sub (as_seq h0 b) 0 32 in
-	  let xResult = Lib.Sequence.sub (as_seq h1 result) 1 32 in
-	let y = Lib.Sequence.sub (as_seq h0 b) 32 32 in
-	  let yResult = Lib.Sequence.sub (as_seq h1 result) 33 32 in
-	uint_v id == 4 /\ xResult == x /\ yResult == y
-      )
-    )
 
-inline_for_extraction
-val compressionCompressedForm: b: lbuffer uint8 (size 64) -> result: compressedForm ->
-  Stack unit
-    (requires fun h -> live h b /\ live h result /\ disjoint b result)
-    (ensures fun h0 _ h1 -> modifies (loc result) h0 h1 /\
-      (
-        let identifier = Lib.Sequence.index (as_seq h1 result) 0 in
-        let x = Lib.Sequence.sub (as_seq h0 b) 0 32 in
-	  let xResult = Lib.Sequence.sub (as_seq h1 result) 1 32 in
-        let y = Lib.Sequence.sub (as_seq h0 b) 32 32 in
-        uint_v identifier == (Lib.ByteSequence.nat_from_intseq_be y % pow2 1)  + 2 /\
-	x == xResult
-      )
-  )
+inline_for_extraction noextract
+val raw_to_uncompressed: pk_raw:lbuffer uint8 64ul -> pk:lbuffer uint8 65ul -> Stack unit
+  (requires fun h -> live h pk /\ live h pk_raw /\ disjoint pk pk_raw)
+  (ensures fun h0 _ h1 -> modifies (loc pk) h0 h1 /\
+    as_seq h1 pk == S.pk_uncompressed_from_raw (as_seq h0 pk_raw))
+
+
+inline_for_extraction noextract
+val raw_to_compressed: pk_raw:lbuffer uint8 64ul -> pk:lbuffer uint8 33ul -> Stack unit
+  (requires fun h -> live h pk /\ live h pk_raw /\ disjoint pk pk_raw)
+  (ensures  fun h0 _ h1 -> modifies (loc pk) h0 h1 /\
+    as_seq h1 pk == S.pk_compressed_from_raw (as_seq h0 pk_raw))
