code/ecdsap256/Hacl.P256.fsti
@@ -9,7 +9,6 @@ open Lib.IntTypes
 open Lib.Buffer
 
 open Spec.Hash.Definitions
-open Hacl.Impl.P256.Compression
 
 module S = Spec.P256
 module BSeq = Lib.ByteSequence
@@ -246,7 +245,7 @@ Comment "Convert 65-byte uncompressed to raw.
   • pk: uint8 [65]
   • pk_raw: uint8 [64]
   Output: bool, where true stands for the correct decompression."]
-val uncompressed_to_raw: pk:notCompressedForm -> pk_raw:lbuffer uint8 64ul -> Stack bool
+val uncompressed_to_raw: pk:lbuffer uint8 65ul -> pk_raw:lbuffer uint8 64ul -> Stack bool
   (requires fun h -> live h pk /\ live h pk_raw /\ disjoint pk pk_raw)
   (ensures fun h0 b h1 -> modifies (loc pk_raw) h0 h1 /\
     (b <==> Some? (S.pk_uncompressed_to_raw (as_seq h0 pk))) /\
@@ -261,7 +260,7 @@ val uncompressed_to_raw: pk:notCompressedForm -> pk_raw:lbuffer uint8 64ul -> St
   • pk: uint8 [33]
   • pk_raw: uint8 [64]
   Output: bool, where true stands for the correct decompression."]
-val compressed_to_raw: pk:compressedForm -> pk_raw:lbuffer uint8 64ul -> Stack bool
+val compressed_to_raw: pk:lbuffer uint8 33ul -> pk_raw:lbuffer uint8 64ul -> Stack bool
   (requires fun h -> live h pk /\ live h pk_raw /\ disjoint pk pk_raw)
   (ensures  fun h0 b h1 -> modifies (loc pk_raw) h0 h1 /\
     (b <==> Some? (S.pk_compressed_to_raw (as_seq h0 pk))) /\
@@ -275,7 +274,7 @@ val compressed_to_raw: pk:compressedForm -> pk_raw:lbuffer uint8 64ul -> Stack b
   Input:
   • pk_raw: uint8 [64]
   • pk: uint8 [65]"]
-val raw_to_uncompressed: pk_raw:lbuffer uint8 64ul -> pk:notCompressedForm -> Stack unit
+val raw_to_uncompressed: pk_raw:lbuffer uint8 64ul -> pk:lbuffer uint8 65ul -> Stack unit
   (requires fun h -> live h pk /\ live h pk_raw /\ disjoint pk pk_raw)
   (ensures fun h0 _ h1 -> modifies (loc pk) h0 h1 /\
     as_seq h1 pk == S.pk_uncompressed_from_raw (as_seq h0 pk_raw))
@@ -285,7 +284,7 @@ val raw_to_uncompressed: pk_raw:lbuffer uint8 64ul -> pk:notCompressedForm -> St
 
   Input: pk_raw: uint8 [64]
   Output: pk: uint8 [33]"]
-val raw_to_compressed: pk_raw:lbuffer uint8 64ul -> pk:compressedForm -> Stack unit
+val raw_to_compressed: pk_raw:lbuffer uint8 64ul -> pk:lbuffer uint8 33ul -> Stack unit
   (requires fun h -> live h pk /\ live h pk_raw /\ disjoint pk pk_raw)
   (ensures  fun h0 _ h1 -> modifies (loc pk) h0 h1 /\
     as_seq h1 pk == S.pk_compressed_from_raw (as_seq h0 pk_raw))
